

1

$$f(t) = f(t + T) \quad \omega_0 = \frac{2\pi}{T}$$

1.1

-

$$f(t) = a_0 + \sum_{n=1}^{\infty} [a_n \cos(n\omega_0 t) + b_n \sin(n\omega_0 t)]$$

-

$$f(t) = \sum_{n=-\infty}^{\infty} c_n e^{jn\omega_0 t}$$

$$c_n = \frac{1}{T} \int_T f(t) e^{-jn\omega_0 t} dt$$

1.2

- $f(t)$

$$c_0 = a_0, \quad c_n = \frac{a_n - jb_n}{2}, \quad c_{-n} = c_n^* \int_{-\infty}^{\infty} |f(t)|^2 dt = \frac{1}{2\pi} \int_{-\infty}^{\infty} |F(\omega)|^2 d\omega$$

$$\begin{aligned} -af(t) + bg(t) &\leftrightarrow ac_n + bd_n \\ f(t - t_0) &\leftrightarrow c_n e^{-jn\omega_0 t_0} \\ f(t) &\Rightarrow \\ c_{-n} &= c_n^* \end{aligned}$$

$$\frac{1}{T} \int_T |f(t)|^2 dt = \sum_{n=-\infty}^{\infty} |c_n|^2$$

2

2.1

-

$$F(\omega) = \mathcal{F}[f(t)] = \int_{-\infty}^{\infty} f(t) e^{-j\omega t} dt$$

-

$$f(t) = \mathcal{F}^{-1}[F(\omega)] = \frac{1}{2\pi} \int_{-\infty}^{\infty} F(\omega) e^{j\omega t} d\omega$$

2.2

$$\begin{aligned} 1. \quad \mathcal{F}[af(t) + bg(t)] &= aF(\omega) + bG(\omega) \\ 2. \quad \mathcal{F}[f(t - t_0)] &= F(\omega) e^{-j\omega t_0} \\ 3. \quad \mathcal{F}[f(t) e^{j\omega_0 t}] &= F(\omega - \omega_0) \\ 4. \quad \mathcal{F}[f(at)] &= \frac{1}{|a|} F\left(\frac{\omega}{a}\right) \\ 5. \quad \mathcal{F}[F(t)] &= 2\pi f(-\omega) \\ 6. \quad \mathcal{F}\left[\frac{d^n f(t)}{dt^n}\right] &= (j\omega)^n F(\omega) \\ 7. \quad \mathcal{F}[t^n f(t)] &= j^n \frac{d^n F(\omega)}{d\omega^n} \\ 8. \quad \mathcal{F}\left[\int_{-\infty}^t f(\tau) d\tau\right] &= \frac{F(\omega)}{j\omega} + \pi F(0) \delta(\omega) \\ 9. \quad \mathcal{F}[f(t) * g(t)] &= F(\omega) G(\omega) \\ 10. \quad \mathcal{F}[f(t)g(t)] &= \frac{1}{2\pi} F(\omega) * G(\omega) \\ 11. \end{aligned}$$

$$12. \quad f(t) \quad F(-\omega) = F^*(\omega)$$

2.3

$$\begin{aligned} -f(t) &\Rightarrow F(\omega) \\ -f(t) &\Rightarrow F(\omega) \\ f(t) &\Rightarrow F(\omega) \\ -f(t) &\Rightarrow F(\omega) \end{aligned}$$

2.4

$$\begin{aligned} -f_e(t) &= \frac{f(t) + f(-t)}{2} \Leftrightarrow F_e(\omega) = \text{Re}\{F(\omega)\} \\ -f_o(t) &= \frac{f(t) - f(-t)}{2} \Leftrightarrow F_o(\omega) = j\text{Im}\{F(\omega)\} \\ -f(t) &= f_e(t) + f_o(t) \\ F(\omega) &= F_e(\omega) + F_o(\omega) \end{aligned}$$

2.5

$$\begin{aligned} \int_{-\infty}^{\infty} |f(t)|^2 dt &= \int_{-\infty}^{\infty} |F(\omega)|^2 d\omega \\ \frac{1}{T} \int_T |f(t)|^2 dt &= \sum_{n=-\infty}^{\infty} |c_n|^2 \\ P &= \lim_{T \rightarrow \infty} \frac{1}{T} \int_{-T/2}^{T/2} |f(t)|^2 dt \end{aligned}$$

2.6

$$\delta(t) \leftrightarrow 1$$

$$1 \leftrightarrow 2\pi\delta(\omega)$$

$$e^{j\omega_0 t} \leftrightarrow 2\pi\delta(\omega - \omega_0)$$

$$\cos(\omega_0 t) \leftrightarrow \pi[\delta(\omega - \omega_0) + \delta(\omega + \omega_0)]$$

$$\sin(\omega_0 t) \leftrightarrow j\pi[\delta(\omega + \omega_0) - \delta(\omega - \omega_0)]$$

$$e^{-at} u(t) \leftrightarrow \frac{1}{a + j\omega} \quad (a > 0)$$

$$te^{-at} u(t) \leftrightarrow \frac{1}{(a + j\omega)^2} \quad (a > 0)$$

$$e^{-a|t|} \leftrightarrow \frac{2a}{a^2 + \omega^2} \quad (a > 0)$$

$$u(t) \leftrightarrow \pi\delta(\omega) + \frac{1}{j\omega}$$

$$\text{rect}\left(\frac{t}{\tau}\right) \leftrightarrow \tau \cdot \frac{\sin(\omega\tau/2)}{\omega\tau/2}$$

$$\text{sinc}(t) = \frac{\sin(\pi t)}{\pi t} \leftrightarrow \text{rect}\left(\frac{\omega}{2\pi}\right)$$

$$\text{tri}\left(\frac{t}{\tau}\right) \leftrightarrow \tau \cdot \frac{\sin^2(\omega\tau/2)}{(\omega\tau/2)^2}$$

$$\sum_{n=-\infty}^{\infty} \delta(t - nT) \leftrightarrow \frac{2\pi}{T} \sum_{k=-\infty}^{\infty} \delta(\omega - k\omega_0)$$

2.7

$$f(t) = \sum_{n=-\infty}^{\infty} c_n e^{jn\omega_0 t}$$

$$F(\omega) = 2\pi \sum_{n=-\infty}^{\infty} c_n \delta(\omega - n\omega_0)$$

$$f(t) = \sum_{k=-\infty}^{\infty} f_0(t - kT)$$

$$F(\omega) = F_0(\omega) \cdot \frac{2\pi}{T} \sum_{n=-\infty}^{\infty} \delta(\omega - n\omega_0)$$

$$c_n = \frac{1}{T} F_0(n\omega_0)$$

3 (DTFT)

3.1

$$x[n] = \mathcal{F}_d^{-1}[X(e^{j\omega})] = \frac{1}{2\pi} \int_{-\pi}^{\pi} X(e^{j\omega}) e^{j\omega n} d\omega$$

3.2

$$\begin{aligned} -\mathcal{F}_d[ax[n] + by[n]] &= aX(e^{j\omega}) + bY(e^{j\omega}) \\ -\mathcal{F}_d[x[n - n_0]] &= e^{-j\omega n_0} X(e^{j\omega}) \\ -\mathcal{F}_d[e^{j\omega_0 n} x[n]] &= X(e^{j(\omega - \omega_0)}) \\ -X(e^{j(\omega + 2\pi)}) &= X(e^{j\omega}) \\ -X[n] &= X^*(e^{j\omega}) \\ -\mathcal{F}_d[nx[n]] &= j \frac{dX(e^{j\omega})}{d\omega} \\ -x_k[n] &= X_k(e^{j\omega}) = X(e^{jk\omega}) \\ \mathcal{F}_d[x[n] * y[n]] &= X(e^{j\omega}) Y(e^{j\omega}) \\ \mathcal{F}_d[x[n]y[n]] &= \frac{1}{2\pi} X(e^{j\omega}) * Y(e^{j\omega}) \end{aligned}$$

3.3

$$\begin{aligned} -x[n] &\Rightarrow X(e^{j\omega}) \\ -x[n] &\Rightarrow X(e^{j\omega}) \end{aligned}$$

3.4 DTFT

$$\delta[n] \leftrightarrow 1$$

$$\delta[n - n_0] \leftrightarrow e^{-j\omega n_0}$$

$$a^n u[n] \leftrightarrow \frac{1}{1 - ae^{-j\omega}} \quad (|a| < 1)$$

$$u[n] \leftrightarrow \frac{1}{1 - e^{-j\omega}} + \pi \sum_{k=-\infty}^{\infty} \delta(\omega - 2\pi k)$$

$$\text{rect}_N[n] \leftrightarrow \frac{\sin(\omega N/2)}{\sin(\omega/2)} e^{-j\omega(N-1)/2}$$

4

4.1

$$F(s) = \mathcal{L}[f(t)] = \int_{-\infty}^{\infty} f(t) e^{-st} dt, \quad s = \sigma + j\omega$$

4.2

$$\begin{aligned} -\mathcal{L}[af(t) + bg(t)] &= aF(s) + bG(s) \\ -\mathcal{L}[f(t - t_0)] &= e^{-st_0} F(s) \\ -\mathcal{L}[e^{-at} f(t)] &= F(s + a) \\ -\mathcal{L}[f(at)] &= \frac{1}{|a|} F\left(\frac{s}{a}\right) \\ -\mathcal{L}[f'(t)] &= sF(s) \\ -\mathcal{L}\left[\int_{-\infty}^t f(\tau) d\tau\right] &= -\frac{F(s)}{s} \\ -\mathcal{L}[f(t) * g(t)] &= F(s)G(s) \\ -f(0^+) &= \lim_{s \rightarrow \infty} sF(s) \\ -\lim_{t \rightarrow \infty} f(t) &= \lim_{s \rightarrow 0} sF(s) \end{aligned}$$

4.3

$$\begin{aligned}\delta(t) &\leftrightarrow 1 \quad (s) \\ u(t) &\leftrightarrow \frac{1}{s} \quad (\operatorname{Re}(s) > 0) \\ -u(-t) &\leftrightarrow \frac{1}{s} \quad (\operatorname{Re}(s) < 0) \\ e^{-at}u(t) &\leftrightarrow \frac{1}{s+a} \quad (\operatorname{Re}(s) > -a) \\ -e^{-at}u(-t) &\leftrightarrow \frac{1}{s+a} \quad (\operatorname{Re}(s) < -a) \\ te^{-at}u(t) &\leftrightarrow \frac{1}{(s+a)^2} \quad (\operatorname{Re}(s) > -a) \\ -te^{-at}u(-t) &\leftrightarrow \frac{1}{(s+a)^2} \quad (\operatorname{Re}(s) < -a) \\ e^{-a|t|} &\leftrightarrow \frac{2a}{s^2 - a^2} \quad (-a < \operatorname{Re}(s) < a) \\ t^n u(t) &\leftrightarrow \frac{n!}{s^{n+1}} \quad (\operatorname{Re}(s) > 0)\end{aligned}$$

5 z

5.1

$$X(z) = \mathcal{Z}[x[n]] = \sum_{n=-\infty}^{\infty} x[n]z^{-n}$$

5.2

$$\begin{aligned}-\mathcal{Z}[ax[n] + by[n]] &= aX(z) + bY(z) \\ \operatorname{ROC} R_1 \cap R_2 - \mathcal{Z}[x[n-n_0]] &= z^{-n_0}X(z) \\ \operatorname{ROC} z = 0 \quad z = \infty \\ -\mathcal{Z}[a^n x[n]] &= X\left(\frac{z}{a}\right) \\ \operatorname{ROC} |z/a| \in R - z \mathcal{Z}[nx[n]] &= -z \frac{dX(z)}{dz} \\ \operatorname{ROC} R - z \mathcal{Z}[x[n]] &= X(z)Y(z) \\ \operatorname{ROC} R_1 \cap R_2 - \mathcal{Z}[x[n] - x[n-1]] &= (1 - z^{-1})X(z) \\ \operatorname{ROC} R \cap \{z \neq 0\} \\ -\mathcal{Z}\left[\sum_{k=-\infty}^n x[k]\right] &= \frac{X(z)}{1-z^{-1}} \\ \operatorname{ROC} R \cap \{|z| > 1\} - x[0] &= \lim_{z \rightarrow \infty} X(z) \\ -\lim_{n \rightarrow \infty} x[n] &= \lim_{z \rightarrow 1} (z - 1)X(z) \quad z = 1\end{aligned}$$

5.3 z

$$\begin{aligned}\delta[n] &\leftrightarrow 1 \quad (z) \\ u[n] &\leftrightarrow \frac{z}{z-1} \quad (|z| > 1) \\ -u[-n-1] &\leftrightarrow \frac{z}{z-1} \quad (|z| < 1) \\ a^n u[n] &\leftrightarrow \frac{z}{z-a} \quad (|z| > |a|) \\ H(s) &= \frac{N(s)}{D(s)} \quad p_i \\ -a^n u[-n-1] &\leftrightarrow \frac{z}{z-a} \quad (|z| < |a|) \\ H(s) &= \sum_i \frac{r_i}{s-p_i}, \quad r_i = [(s-p_i)H(s)]_{s=p_i} \\ na^n u[n] &\leftrightarrow \frac{az}{(z-a)^2} \quad (|z| > |a|) \\ -na^n u[-n-1] &\leftrightarrow \frac{az}{(z-a)^2} \quad (|z| < |a|) \\ \cos(\omega_0 n)u[n] &\leftrightarrow \frac{z(z - \cos \omega_0)}{z^2 - 2z \cos \omega_0 + 1} \\ \sin(\omega_0 n)u[n] &\leftrightarrow \frac{z \sin \omega_0}{z^2 - 2z \cos \omega_0 + 1}\end{aligned}$$

6 LTI

6.1

$$H(s) = \frac{Y(s)}{X(s)} = \mathcal{L}[h(t)]$$

6.2

$$-\operatorname{BIBO} \operatorname{Re}(p_j) < 0 \quad -\operatorname{Re}(p_j) > 0$$

6.3

$$H(j\omega) = H(s) \Big|_{s=j\omega}$$

6.4

$$\begin{aligned}y(t) &= Kx(t - t_d) \\ -|H(j\omega)| &= K - \angle H(j\omega) = -\omega t_d \\ H(j\omega) &= Ke^{-j\omega t_d}\end{aligned}$$

6.5

$$\begin{aligned}-\tau_g(\omega) &= -\frac{d\theta(\omega)}{d\omega} \theta(\omega) = \angle H(j\omega) \\ \tau_p(\omega) &= -\frac{\theta(\omega)}{\omega} - \tau_g = \tau_p = t_d\end{aligned}$$

6.6

$$H(s) = \sum_i \frac{r_i}{s-p_i}, \quad r_i = [(s-p_i)H(s)]_{s=p_i}$$

7 LTI

7.2

$$-\operatorname{BIBO} |p_j| < 1 \quad -|p_j| > 1$$

7.3

$$H(e^{j\omega}) = H(z) \Big|_{z=e^{j\omega}}$$

7.4

$$\sum_{k=0}^N a_k y[n-k] = \sum_{k=0}^M b_k x[n-k]$$

$$H(z) = \frac{Y(z)}{X(z)} = \frac{\sum_{k=0}^M b_k z^{-k}}{\sum_{k=0}^N a_k z^{-k}}$$

8

8.1 s

$$\begin{aligned}-H(s) &\operatorname{ROC} \operatorname{Re}(s) > \sigma_0 - \operatorname{ROC} \operatorname{Re}(p) < 0 \\ -\operatorname{ROC} \operatorname{Re}(s) > \sigma_0 &\sigma_0 < 0\end{aligned}$$

8.2 z

$$\begin{aligned}-\operatorname{ROC} |z| > r - \operatorname{ROC} |z| = 1 \quad |p| < 1 \\ -\operatorname{ROC} |z| > r \quad r < 1\end{aligned}$$

9

$$\begin{aligned}-H(s) &= H_1(s)H_2(s) \quad H(z) = H_1(z)H_2(z) \\ -H(s) &= H_1(s) + H_2(s) \quad H(z) = H_1(z) + H_2(z) \\ -H(s) &= \frac{H_1(s)}{1 \pm H_1(s)H_2(s)} \quad H(z) = \frac{H_1(z)}{1 \pm H_1(z)H_2(z)}\end{aligned}$$

10 z

10.1

$$\begin{aligned}1 - \operatorname{Re}(s) < 0 \quad -|z| < 1 \\ 1 - \operatorname{Re}(s) > 0 \quad -|z| > 1\end{aligned}$$

10.2

$$\begin{aligned}z = e^{sT} \quad s = \frac{1}{T} \ln z \\ -s \quad z - s \quad z - s \quad z - \pi/T < \omega < \pi/T\end{aligned}$$

11

11.1

$$\begin{aligned}-x_p(t) &= x(t) \sum_{n=-\infty}^{\infty} \delta(t - nT) \\ X_p(j\omega) &= \frac{1}{T} \sum_{k=-\infty}^{\infty} X(j(\omega - k\omega_s)), \\ \omega_s &\end{aligned}$$

11.2

$$\begin{aligned}-x(t) \quad \omega_M X(j\omega) = 0, |\omega| > \omega_M \\ \omega_s \geq 2\omega_M\end{aligned}$$

11.3

$$H_r(j\omega) = \begin{cases} T & |\omega| < \omega_c \\ 0 & |\omega| \geq \omega_c \end{cases}, \quad \omega_M < \omega_c < \omega_{M+1}$$

- ZOH

$$x_0(t) = \sum_{n=-\infty}^{\infty} x(nT) \operatorname{rect}\left(\frac{t - nT - T/2}{T}\right)$$

$$\begin{aligned}X_0(j\omega) &= H_0(j\omega)X_p(j\omega) \\ H_0(j\omega) &= T \operatorname{sinc}\left(\frac{\omega T}{2}\right) e^{-j\omega T/2}\end{aligned}$$

$$x_1(t) = \sum_{n=-\infty}^{\infty} x(nT) \operatorname{tri}\left(\frac{t - nT}{T}\right)$$

$$\begin{aligned}X_1(j\omega) &= H_1(j\omega)X_p(j\omega) \\ H_1(j\omega) &= T \operatorname{sinc}^2\left(\frac{\omega T}{2}\right)\end{aligned}$$

11.4

$$1. \quad C/Dx[n] = x_c(nT)$$

$$X(e^{j\omega}) = \frac{1}{T} \sum_{k=-\infty}^{\infty} X_c\left(j\frac{\omega - 2\pi k}{T}\right)$$

$$\begin{aligned}2. \quad Y(e^{j\omega}) &= H(e^{j\omega})X(e^{j\omega}) \\ \Omega &= \omega T \\ 3. \quad D/C - y_c(t) &= \sum_{n=-\infty}^{\infty} y[n] \frac{\sin(\pi(t-nT)/T)}{\pi(t-nT)/T} \\ -y_c(t) &= \sum_{n=-\infty}^{\infty} y[n] \operatorname{rect}\left(\frac{t-nT-T/2}{T}\right) \\ 4. \quad H_{eff}(j\Omega) &= H(e^{j\Omega/T})|\Omega| < \pi/T\end{aligned}$$

$$\begin{aligned}1. \quad \omega_s &\geq 2\omega_M \\ -\omega_s &< 2\omega_M\end{aligned}$$

11.6

$$1. \quad / \quad 2. \quad 3. \quad z$$